newly defined appsub

Haskell.hs
@@ -1,0 +1,17 @@
+{-# LANGUAGE MultiParamTypeClasses #-}
+
+class Addable a b where
+    add :: a -> b -> a
+
+instance Addable Int  Int where
+    add x y = x + y
+
+instance Addable Int Bool where
+    add x y = if y then x + 1 else x
+
+
+ex1 = add (1 :: Int)
+
+-- no parallel here
+
+ex2 = add (1 :: Int) (1 :: Int)
